Updates.

FOL/NV/Alpha/Ind/Alpha.lean
@@ -16,15 +16,13 @@ inductive are_alpha_equiv_ind_v1 : Formula_ → Formula_ → Prop
   | rename_forall_
     (phi : Formula_)
     (x y : VarName_) :
-    ¬ var_is_free_in y phi →
-    ¬ var_is_bound_in y phi →
+    ¬ var_occurs_in y phi →
     are_alpha_equiv_ind_v1 (forall_ x phi) (forall_ y (replace_var_one_rec x y phi))
 
   | rename_exists_
     (phi : Formula_)
     (x y : VarName_) :
-    ¬ var_is_free_in y phi →
-    ¬ var_is_bound_in y phi →
+    ¬ var_occurs_in y phi →
     are_alpha_equiv_ind_v1 (exists_ x phi) (exists_ y (replace_var_one_rec x y phi))
 
   | compat_not_
@@ -89,15 +87,13 @@ inductive are_alpha_equiv_ind_v2 : Formula_ → Formula_ → Prop
   | rename_forall_
     (phi : Formula_)
     (x y : VarName_) :
-    ¬ var_is_free_in y phi →
-    ¬ var_is_bound_in y phi →
+    ¬ var_occurs_in y phi →
     are_alpha_equiv_ind_v2 (forall_ x phi) (forall_ y (Sub.Var.One.Rec.fast_replace_free_var_one_rec x y phi))
 
   | rename_exists_
     (phi : Formula_)
     (x y : VarName_) :
-    ¬ var_is_free_in y phi →
-    ¬ var_is_bound_in y phi →
+    ¬ var_occurs_in y phi →
     are_alpha_equiv_ind_v2 (exists_ x phi) (exists_ y (Sub.Var.One.Rec.fast_replace_free_var_one_rec x y phi))
 
   | compat_not_
@@ -204,12 +200,8 @@ lemma are_alpha_equiv_ind_v1_replace_var_one_rec_fast_replace_free_var_one_rec
         first
           | apply are_alpha_equiv_ind_v1.rename_forall_
           | apply are_alpha_equiv_ind_v1.rename_exists_
-        · simp only [var_is_free_in_iff_mem_free_var_set]
-          apply not_mem_var_set_imp_not_mem_free_var_set
-          exact h1_left
-        · simp only [var_is_bound_in_iff_mem_bound_var_set]
-          apply not_mem_var_set_imp_not_mem_bound_var_set
-          exact h1_left
+        simp only [var_occurs_in_iff_mem_var_set]
+        exact h1_left
       case neg c1 =>
         first
         | apply are_alpha_equiv_ind_v1.compat_forall_
@@ -261,13 +253,9 @@ lemma are_alpha_equiv_ind_v2_fast_replace_free_var_one_rec_replace_var_one_rec
         subst c1
         apply are_alpha_equiv_ind_v2.trans_
         · first
-            | apply are_alpha_equiv_ind_v2.rename_forall_
-            | apply are_alpha_equiv_ind_v2.rename_exists_
-          · simp only [var_is_free_in_iff_mem_free_var_set]
-            apply not_mem_var_set_imp_not_mem_free_var_set
-            exact h1_left
-          · simp only [var_is_bound_in_iff_mem_bound_var_set]
-            apply not_mem_var_set_imp_not_mem_bound_var_set
+            | apply are_alpha_equiv_ind_v2.rename_forall_ phi v t
+            | apply are_alpha_equiv_ind_v2.rename_exists_ phi v t
+          · simp only [var_occurs_in_iff_mem_var_set]
             exact h1_left
         · first
             | apply are_alpha_equiv_ind_v2.compat_forall_
@@ -287,14 +275,13 @@ lemma are_alpha_equiv_ind_v1_imp_are_alpha_equiv_ind_v2
   by
     induction h1
     case
-        rename_forall_ phi x y ih_1 ih_2
-      | rename_exists_ phi x y ih_1 ih_2 =>
+        rename_forall_ phi x y ih_1
+      | rename_exists_ phi x y ih_1 =>
       apply are_alpha_equiv_ind_v2.trans_
       · first
-          | apply are_alpha_equiv_ind_v2.rename_forall_
-          | apply are_alpha_equiv_ind_v2.rename_exists_
-        · exact ih_1
-        · exact ih_2
+          | apply are_alpha_equiv_ind_v2.rename_forall_ phi x y
+          | apply are_alpha_equiv_ind_v2.rename_exists_ phi x y
+        exact ih_1
       · first
           | apply are_alpha_equiv_ind_v2.compat_forall_
           | apply are_alpha_equiv_ind_v2.compat_exists_
@@ -346,8 +333,7 @@ theorem replace_empty_Holds
   (u v : VarName_)
   (F : Formula_)
   (a : D)
-  (h1 : ¬ var_is_free_in v F)
-  (h2 : ¬ var_is_bound_in v F) :
+  (h1 : ¬ var_occurs_in v F) :
   holds D I (Function.updateITE V u a) E F ↔
     holds D I (Function.updateITE V v a) E (Sub.Var.One.Rec.fast_replace_free_var_one_rec u v F) :=
   by
@@ -355,7 +341,7 @@ theorem replace_empty_Holds
   all_goals
     induction F generalizing V
     case pred_const_ X xs | pred_var_ X xs =>
-      simp only [var_is_free_in] at h1
+      simp only [var_occurs_in] at h1
 
       simp only [Sub.Var.One.Rec.fast_replace_free_var_one_rec]
       simp only [holds]
@@ -370,12 +356,12 @@ theorem replace_empty_Holds
       case _ c1 c2 =>
         contradiction
       case _ c1 c2 =>
-        subst c2
+        rw [← c2] at a1
         contradiction
       case _ c1 c2 =>
         rfl
     case eq_ x y =>
-      simp only [var_is_free_in] at h1
+      simp only [var_occurs_in] at h1
 
       simp only [Sub.Var.One.Rec.fast_replace_free_var_one_rec]
       simp only [holds]
@@ -388,69 +374,63 @@ theorem replace_empty_Holds
       simp only [Sub.Var.One.Rec.fast_replace_free_var_one_rec]
       simp only [holds]
     case not_ phi phi_ih =>
-      simp only [var_is_free_in] at h1
-
-      simp only [var_is_bound_in] at h2
+      simp only [var_occurs_in] at h1
 
       simp only [Sub.Var.One.Rec.fast_replace_free_var_one_rec]
       simp only [holds]
       congr! 1
-      exact phi_ih V h1 h2
+      apply phi_ih
+      exact h1
     case
         imp_ phi psi phi_ih psi_ih
       | and_ phi psi phi_ih psi_ih
       | or_ phi psi phi_ih psi_ih
       | iff_ phi psi phi_ih psi_ih =>
-      simp only [var_is_free_in] at h1
-      push_neg at h1
+      simp only [var_occurs_in] at h1
+      simp at h1
+      obtain ⟨h1_left, h1_right⟩ := h1
 
-      simp only [var_is_bound_in] at h2
-      push_neg at h2
-
-      cases h1
-      case intro h1_left h1_right =>
-        cases h2
-        case intro h2_left h2_right =>
-          simp only [Sub.Var.One.Rec.fast_replace_free_var_one_rec]
-          simp only [holds]
-          congr! 1
-          · exact phi_ih V h1_left h2_left
-          · exact psi_ih V h1_right h2_right
+      simp only [Sub.Var.One.Rec.fast_replace_free_var_one_rec]
+      simp only [holds]
+      congr! 1
+      · exact phi_ih V h1_left
+      · exact psi_ih V h1_right
     case forall_ x phi phi_ih | exists_ x phi phi_ih =>
-      simp only [var_is_free_in] at h1
-      push_neg at h1
+      simp only [var_occurs_in] at h1
+      simp at h1
+      obtain ⟨h1_left, h1_right⟩ := h1
 
-      simp only [var_is_bound_in] at h2
-      push_neg at h2
+      simp only [Sub.Var.One.Rec.fast_replace_free_var_one_rec]
+      split_ifs
+      case pos c1 =>
+        rw [c1]
 
-      cases h2
-      case intro h2_left h2_right =>
-        simp only [Sub.Var.One.Rec.fast_replace_free_var_one_rec]
-        split_ifs
-        case pos c1 =>
-          subst c1
-          apply holds_coincide_var
-          intro x a1
-          simp only [var_is_free_in] at a1
-          cases a1
-          case h1.intro a1_left a1_right =>
-            simp only [Function.updateITE]
-            simp only [if_neg a1_left]
-            split_ifs
-            case pos c2 =>
-              subst c2
-              tauto
-            case neg c2 =>
-              rfl
-        case neg c1 =>
-          simp only [holds]
-          first | apply forall_congr' | apply exists_congr
-          intro d
-          simp only [Function.updateITE_comm V v x d a h2_left]
-          simp only [Function.updateITE_comm V u x d a c1]
-          apply phi_ih
-          · exact h1 h2_left
-          · exact h2_right
+        apply holds_coincide_var
+        intro y a1
+        simp only [var_is_free_in] at a1
+        obtain ⟨a1_left, a1_right⟩ := a1
+
+        simp only [var_occurs_in_iff_var_is_bound_in_or_var_is_free_in] at h1_right
+        simp at h1_right
+        obtain ⟨h1_right_left, h1_right_right⟩ := h1_right
+
+        have s1 : ¬ y = v :=
+        by
+          intro contra
+          apply h1_right_right
+          rw [← contra]
+          exact a1_right
+
+        simp only [Function.updateITE]
+        split_ifs <;> rfl
+      case neg c1 =>
+        simp only [holds]
+        first | apply forall_congr' | apply exists_congr
+        intro d
+        simp only [Function.updateITE_comm V v x d a h1_left]
+        simp only [Function.updateITE_comm V u x d a c1]
+        apply phi_ih
+        exact h1_right
   case nil.def_ X xs =>
     simp only [Sub.Var.One.Rec.fast_replace_free_var_one_rec]
     simp only [holds]
@@ -462,7 +442,7 @@ theorem replace_empty_Holds
       case _ =>
         simp
       case _ c1 =>
-        simp only [var_is_free_in] at h1
+        simp only [var_occurs_in] at h1
 
         apply holds_coincide_var
         intro v' a1
@@ -499,8 +479,7 @@ theorem replace_empty_Holds
             exact c1_right
       case _ =>
         apply ih
-        · exact h1
-        · exact h2
+        exact h1
 
 
 theorem Holds_iff_alphaEqv_Holds
@@ -513,11 +492,12 @@ theorem Holds_iff_alphaEqv_Holds
   holds D I V E F ↔ holds D I V E F' :=
   by
   induction h1 generalizing V
-  case rename_forall_ h1_phi h1_x h1_y h1_1 h1_2 | rename_exists_ h1_phi h1_x h1_y h1_1 h1_2 =>
+  case rename_forall_ h1_phi h1_x h1_y h1_1 | rename_exists_ h1_phi h1_x h1_y h1_1 =>
     simp only [holds]
     first | apply forall_congr' | apply exists_congr
     intro d
-    exact replace_empty_Holds D I V E h1_x h1_y h1_phi d h1_1 h1_2
+    apply replace_empty_Holds
+    exact h1_1
   case compat_not_ h1_phi h1_phi' _ h1_ih =>
     simp only [holds]
     congr! 1
